theories/heap_lang/lib/membrane.v
@@ -1,0 +1,389 @@
+From iris.heap_lang Require Export heap.
+From iris.heap_lang Require notation.
+From iris.proofmode Require Import tactics.
+From iris.heap_lang Require Import proofmode.
+Import uPred.
+
+(** * Membrane code *)
+(**
+	The membrane constructs values that may be safely shared with
+	adversarial code (i.e., values in [lowval ≡ on_val lowloc]).
+
+	To read the code, it helps to have a spec in mind. Roughly,
+	our specification says that if [locout : Ψ → lowloc] and
+	[locin : lowloc → Ψ] for some "type" [Ψ] of locations, then
+	[membrane locout locin : on_val Ψ → on_val lowloc]; that is,
+	the membrane lifts reference monitors for locations to
+	reference monitors for values. See [membrane_spec] and the
+	special case [inert_membrane_spec].
+*)
+Section code.
+  Import notation.
+  Definition membrane : val := rec: "membrane" "locout" "locin" "x" :=
+    let: "wrap" := "membrane" "locout" "locin" in
+    iffun: "x" as "f" =>
+      let: "unwrap" := "membrane" "locin" "locout" in
+      λ: "y", "wrap" ("f" ("unwrap" "y"))
+    else iflit: "x" as "lit" =>
+      ifloc: "lit" as "l" => "locout" "l" else "lit"
+    else ifpair: "x" as "p" =>
+      let: "v1" := "wrap" (Fst "p") in
+      let: "v2" := "wrap" (Snd "p") in
+      ("v1", "v2")
+    else ifinl: "x" as "x" => InjL ("wrap" "x")
+    else ifinr: "x" as "x" => InjR ("wrap" "x")
+    else assert: #false.
+End code.
+
+(**
+	The membrane's main ingredient is its treatment of functions.
+	(We made some inessential choices in writing this code. One
+	need not preserve the structure of values or only apply
+	reference monitors to locations.)
+
+	The membrane does not offer unconditional safety. It avoids
+	leaking high values to the adversary, but does not prevent the
+	adversary from applying wrapped functions to "wrong" inputs,
+	which is another way to interfere with otherwise safe code.
+	The function [two ≔ λ r, assert (!r = 2)], for example, may be
+	safely applied to any location containing the value 2 and to
+	any non-location. In general, we may share neither [two] nor
+	[wrap two] with the adversary. To see that [two] is unsafe,
+	pick [C[•] := • (ref 1)]. To see that [wrap two] is unsafe,
+	assume locations [ℓ], [ℓ'] such that [ℓ] is low and [locin ℓ]
+	returns [ℓ'] and [ℓ'] contains the value 1. (This situation
+	can easily arise when [locin] and [locout] maintain a partial
+	bijection on locations and some verified code wraps [ℓ'].)
+	Now, pick [C[•] := • ℓ].
+
+	So, any membrane spec must make an assumption about the value
+	to be wrapped. To verify the function case, any such
+	assumption must imply WP for the bodies of wrapped functions.
+	Can we use a simple syntactic restriction and, internally, a
+	logical relation to obtain the necessary WP? Yes, but there is
+	little point. If our restriction implies syntactic lowness,
+	then the robust safety theorem says every restricted
+	expression is semantically low, and the membrane buys us
+	nothing. Now, our restriction *must* imply syntactic lowness.
+	Our restriction must rule out assertions as the function [wrap
+	(λ_. assert false)] is unsafe. Our restriction must rule out
+	high locations (or heap operations, a non-starter). This is
+	necessary because, to prove the FTLR, we must show that if [ℓ]
+	is compatible, so is [! ℓ], and we're working under the heap
+	invaraint.
+*)
+
+(** * Reference monitors *)
+(**
+	The assertion [is_mon v Ψ1 Ψ2] means that [v] is a reference
+	monitor of "type" [Ψ1 → Ψ2] where the [Ψ_i] are predicates on
+	some type [A] that may be injected into values. (We care about
+	[A = loc] and [A = val].)
+*)
+Section is_mon.
+  Context `{heapG Σ} {A : Type} (f : A → val).
+  Notation ext R := (pointwise_relation _ R).
+
+  Definition is_mon (v : val) (Ψ1 Ψ2 : A → iProp Σ) : iProp Σ :=
+    (∀ a, {{{ Ψ1 a }}} v (f a) ?{{{ a, RET f a; Ψ2 a }}})%I.
+
+  Global Instance is_mon_persistent v Ψ1 Ψ2 :
+    PersistentP (is_mon v Ψ1 Ψ2).
+  Proof. apply _. Qed.
+  Global Instance is_mon_ne v n :
+     Proper (ext (dist n) ==> ext (dist n) ==> dist n) (is_mon v).
+  Proof. solve_proper. Qed.
+  Global Instance is_mon_proper v :
+     Proper (ext (≡) ==> ext (≡) ==> (≡)) (is_mon v).
+  Proof. solve_proper. Qed.
+End is_mon.
+Typeclasses Opaque is_mon.
+
+(** * Lifting location predicates to value predicates *)
+(**
+	Given a predicate [Ψ] on locations, the predicate [lift Ψ] on
+	values lifts [Ψ] structurally. If [Ψ] is persistent, so is
+	[lift Ψ].
+
+	Introduction: Lifted values (i) include all locations
+	satisfying [Ψ] and all other base values and (ii) are closed
+	under function abstraction, pairing, and injections.
+
+	Elimination: Heap resources for lifted locations are
+	determined by [Ψ]; otherwise, eliminating a lifted value
+	produces a lifted value.
+
+	For the membrane verification, the salient point is that [lift
+	Ψ (Rec f x e)] comprises a weakest-precondition for [e].
+*)
+Section lift.
+  Context `{heapG Σ} (Ψ : loc → iProp Σ).
+
+  Definition lift_pre (rec : val -c> iProp Σ) : val -c> iProp Σ := λ v,
+    match v with
+    | RecV f x e _ => □ ▷ ∀ v Φ, rec v -∗ (∀ v, rec v -∗ Φ v) -∗
+      WP subst' x (of_val v) (subst' f (Rec f x e) e) ?{{ Φ }}
+    | LitV (LitLoc l) => Ψ l
+    | LitV (LitInt _ | LitBool _ | LitUnit) => True
+    | PairV v1 v2 => ▷(rec v1 ∗ rec v2)
+    | InjLV v | InjRV v => ▷(rec v)
+    end%I.
+
+  Instance lift_pre_contractive : Contractive lift_pre.
+  Proof.
+    rewrite /lift_pre=> n rec rec' Hrec ?.
+    repeat (f_contractive || f_equiv); apply Hrec.
+  Qed.
+
+  Definition lift : val → iProp Σ := fixpoint lift_pre.
+
+  Lemma lift_unfold v : lift v ≡ lift_pre lift v.
+  Proof. exact: (fixpoint_unfold lift_pre). Qed.
+
+  Global Instance lift_persistent v :
+    (∀ l, PersistentP (Ψ l)) → PersistentP (lift v).
+  Proof.
+    move=>Hloc. iIntros "Hv". iLöb as "IH" forall (v).
+    rewrite lift_unfold. case: v.
+    - intros. by iDestruct "Hv" as "#Hv".
+    - by case; intros; iDestruct "Hv" as "#Hv".
+    - intros. rewrite always_later. iNext. iDestruct "Hv" as "(Hv1&Hv2)".
+      iDestruct ("IH" with "* Hv1") as "#Hv1'". iClear "Hv1".
+      iDestruct ("IH" with "* Hv2") as "#Hv2'". iClear "Hv2".
+      iAlways. by iFrame "#".
+    - intros. rewrite always_later. iNext.
+      by iSpecialize ("IH" with "* Hv").
+    - intros. rewrite always_later. iNext.
+      by iSpecialize ("IH" with "* Hv").
+  Qed.
+
+  Lemma lift_elim v :
+    lift v ⊣⊢
+    match v with
+    | RecV f x e _ => □ ▷ ∀ v Φ, lift v -∗ (∀ v, lift v -∗ Φ v) -∗
+      WP subst' x (of_val v) (subst' f (Rec f x e) e) ?{{ Φ }}
+    | LitV (LitLoc l) => Ψ l
+    | LitV (LitInt _ | LitBool _ | LitUnit) => True
+    | PairV v1 v2 => ▷(lift v1 ∗ lift v2)
+    | InjLV v | InjRV v => ▷(lift v)
+    end%I.
+  Proof. rewrite lift_unfold. by case: v. Qed.
+End lift.
+Typeclasses Opaque lift.
+
+(** * Membrane proof *)
+
+Section proof.
+  Import notation.
+  Context `{heapG Σ} (locin locout : val) (Ψ : loc → iProp Σ).
+  Context {HΨ : ∀ l, PersistentP (Ψ l)}.
+  Notation of_loc := (λ l : loc, #l).
+
+  Lemma wrap_unwrap :
+    is_mon of_loc locout Ψ low -∗
+    is_mon of_loc locin low Ψ -∗
+    □ ((∀ p E Φ, ▷(∀ v, is_mon id v (lift Ψ) low -∗ Φ v) -∗
+      WP membrane locout locin @ p; E {{ Φ }}) ∗
+     (∀ p E Φ, ▷(∀ v, is_mon id v low (lift Ψ) -∗ Φ v) -∗
+      WP membrane locin locout @ p; E {{ Φ }}))%I.
+  Proof.
+    iIntros "#Hlocout #Hlocin".
+    iLöb as "IH". iDestruct "IH" as "#(IHmkw & IHmku)".
+      do 2!rewrite -always_later always_elim. iAlways.
+    iSplitL.
+    - iIntros (p E Φ) "HΦ". wp_rec. wp_lam.
+      iApply "HΦ". clear Φ. iIntros (v) "!#". iIntros (Φ) "#Hv HΦ". wp_lam.
+      wp_apply "IHmkw". iIntros (wrap) "#Hwrap". iClear "IHmkw".
+        rewrite {4}/is_mon. setoid_rewrite always_elim. wp_let.
+
+      (* Wrapping functions. *)
+      wp_typecast Hrec.
+      + iClear "Hlocout Hlocin".
+        (* Unfold Hv early, to eat the later. *)
+        destruct (is_rec_val _ Hrec) as (f&x&erec&?&->).
+          rewrite lift_elim always_elim. wp_match.
+        wp_apply "IHmku". iIntros (unwrap) "#Hunwrap". iClear "IHmku".
+          rewrite/is_mon. wp_let.
+        iApply "HΦ". clear Φ.
+        rewrite low_rec. iAlways. iNext. iIntros (v1 Φ) "Hv1 HΦ".
+          simpl_subst.
+        wp_apply ("Hunwrap" with "* [$Hv1]"). iIntros (v2) "Hv2". wp_rec.
+        wp_apply ("Hv" with "[$Hv2]"). iIntros (v3) "Hv3".
+        by wp_apply ("Hwrap" with "* [$Hv3]").
+      wp_match. iClear "IHmku Hlocin".
+
+      (* Wrapping literals. *)
+      wp_typecast Hlit; wp_match.
+      + iClear "Hwrap".
+
+        (* Wrapping locations. *)
+        wp_typecast Hloc; wp_match.
+        * destruct (is_loc_val _ Hloc) as (l&->). rewrite lift_elim /is_mon.
+          wp_apply ("Hlocout" with "* [$Hv]"). iIntros (v1) "Hv1".
+          iApply "HΦ". by rewrite low_val.
+
+        (* Wrapping other literals. *)
+        iApply "HΦ". destruct (is_lit_val _ Hlit) as (lit&HV).
+          rewrite HV low_val. rewrite HV /is_loc in Hloc.
+        case: lit Hloc {Hlit HV} => // l Hloc. by exfalso; eauto.
+      iClear "Hlocout".
+
+      (* Wrapping pairs. *)
+      wp_typecast Hp.
+      + (* Unfold Hv early, to eat the later. *)
+        destruct (is_pair_val _ Hp) as (v1&v2&->).
+          rewrite lift_elim. iDestruct "Hv" as "#(Hv1 & Hv2)".
+          wp_match. wp_proj.
+        wp_apply ("Hwrap" with "* [$Hv1]"). iIntros (v'1) "Hv'1". wp_let.
+          wp_proj.
+        wp_apply ("Hwrap" with "* [$Hv2]"). iIntros (v'2) "Hv'2". wp_let.
+        iApply "HΦ". rewrite (low_val (PairV _ _)). by iFrame.
+      wp_match.
+
+      (* Wrapping left injections. *)
+      wp_typecast v0 Hinl.
+      + (* Unfold Hv early, to eat the later. *)
+        rewrite Hinl lift_elim. wp_match.
+        wp_apply ("Hwrap" with "* [$Hv]"). iIntros (v1) "Hv1". wp_value.
+        iApply "HΦ". rewrite (low_val (InjLV _)). by iFrame.
+      wp_match.
+
+      (* Wrapping right injections. *)
+      wp_typecast v0 Hinr.
+      + (* Unfold Hv early, to eat the later. *)
+        rewrite Hinr lift_elim. wp_match.
+        wp_apply ("Hwrap" with "* [$Hv]"). iIntros (v1) "Hv1". wp_value.
+        iApply "HΦ". rewrite (low_val (InjRV _)). by iFrame.
+      wp_match.
+      iExFalso. iPureIntro. exact: is_val_exhaustive.
+
+    - iIntros (p E Φ) "HΦ". wp_rec. wp_lam.
+      iApply "HΦ". clear Φ. iIntros (v) "!#". iIntros (Φ) "#Hv HΦ". wp_lam.
+      wp_apply "IHmku". iIntros (unwrap) "#Hunwrap". iClear "IHmku".
+        rewrite {4}/is_mon. setoid_rewrite always_elim. wp_let.
+
+      (* Unwrapping functions. *)
+      wp_typecast Hrec.
+      + iClear "Hlocout Hlocin".
+        (* Unfold Hv early, to eat the later. *)
+        destruct (is_rec_val v Hrec) as (f&x&erec&?&->).
+          rewrite low_rec always_elim. wp_match.
+        wp_apply "IHmkw". iIntros (wrap) "#Hwrap". iClear "IHmkw".
+          rewrite/is_mon. wp_let.
+        iApply "HΦ". clear Φ.
+        rewrite lift_elim. iAlways. iNext. iIntros (v1 Φ) "Hv1 HΦ".
+          simpl_subst.
+        wp_apply ("Hwrap" with "* [$Hv1]"). iIntros (v2) "Hv2". wp_rec.
+        wp_apply ("Hv" with "[$Hv2]"). iIntros (v3) "Hv3".
+        by wp_apply ("Hunwrap" with "* [$Hv3]").
+      wp_match. iClear "IHmkw Hlocout".
+
+      (* Unwrapping literals. *)
+      wp_typecast Hlit; wp_match.
+      + iClear "Hunwrap".
+
+        (* Unwrapping locations. *)
+        wp_typecast Hloc; wp_match.
+        * destruct (is_loc_val _ Hloc) as (l1&->). rewrite low_val /is_mon.
+          wp_apply ("Hlocin" with "* [$Hv]"). iIntros (l2) "Hl2".
+          iApply "HΦ". by rewrite lift_elim.
+
+        (* Unwrapping other literals. *)
+        iApply "HΦ". destruct (is_lit_val _ Hlit) as (lit&HV).
+          rewrite HV lift_elim. rewrite HV /is_loc in Hloc.
+        case: lit Hloc {Hlit HV} => // l Hloc. by exfalso; eauto.
+      iClear "Hlocin".
+
+      (* Unwrapping pairs. *)
+      wp_typecast Hp.
+      + (* Unfold Hv early, to eat the later. *)
+        destruct (is_pair_val _ Hp) as (v1&v2&->).
+          rewrite (low_val (PairV _ _)). iDestruct "Hv" as "#(Hv1 & Hv2)".
+          wp_match. wp_proj.
+        wp_apply ("Hunwrap" with "* [$Hv1]"). iIntros (v'1) "Hv'1". wp_let.
+          wp_proj.
+        wp_apply ("Hunwrap" with "* [$Hv2]"). iIntros (v'2) "Hv'2". wp_let.
+        iApply "HΦ". rewrite (lift_elim _ (PairV _ _)). by iFrame.
+      wp_match.
+
+      (* Unwrapping left injections. *)
+      wp_typecast v0 Hinl.
+      + (* Unfold Hv early, to eat the later. *)
+        rewrite Hinl (low_val (InjLV _)). wp_match.
+        wp_apply ("Hunwrap" with "* [$Hv]"). iIntros (v1) "Hv1". wp_value.
+        iApply "HΦ". rewrite (lift_elim _ (InjLV _)). by iFrame.
+      wp_match.
+
+      (* Unwrapping right injections. *)
+      wp_typecast v0 Hinr.
+      + (* Unfold Hv early, to eat the later. *)
+        rewrite Hinr (low_val (InjRV _)). wp_match.
+        wp_apply ("Hunwrap" with "* [$Hv]"). iIntros (v1) "Hv1". wp_value.
+        iApply "HΦ". rewrite (lift_elim _ (InjRV _)). by iFrame.
+      wp_match.
+      iExFalso. iPureIntro. exact: is_val_exhaustive.
+  Qed.
+
+  (**
+	The membrane lifts reference monitors (of type [Ψ ↔ low]) on
+	locations to reference monitors (of type [lift Ψ → low]) on
+	values.
+  *)
+  Lemma membrane_spec p E :
+    {{{ is_mon of_loc locout Ψ low ∗ is_mon of_loc locin low Ψ }}}
+      membrane locout locin @ p; E
+    {{{ wrap, RET wrap; is_mon id wrap (lift Ψ) low }}}.
+  Proof.
+    iIntros (Φ) "[Hout Hin] HΦ".
+    iDestruct (wrap_unwrap with "[$Hout] [$Hin]") as "(Hw & _)".
+    by iApply "Hw".
+  Qed.
+End proof.
+
+(**
+	When [locout] works unconditionally, the membrane can wrap all
+	_inert_ values. Inert values (i) include all base values and
+	(ii) are closed under function abstraction, pairing, and
+	injections. Inert locations cannot be used to inspect or
+	modify the heap; otherwise, eliminating an inert value
+	produces an inert value.
+
+	Examples:
+
+	[λ _, ℓ] is inert, whether location ℓ is high or low
+
+	[λ x, assert (x = 1)] is not inert because, if x is any inert
+	value, there is no way to prove x = 1
+
+	[λ x, ! x] is not inert because inert locations cannot inspect
+	the heap
+
+	[λ x, assume (x = ℓ); ! x; ()] is inert (assuming, say, a
+	suitable invariant about location ℓ)
+*)
+Section inert.
+  Context `{heapG Σ}.
+  Implicit Types l : loc.
+  Implicit Types v : val.
+  Import notation.
+
+  Definition inert : val → iProp Σ := on_val (const True%I).
+  Definition is_locout (locout : val) : iProp Σ :=
+    (∀ l1, {{{ True }}} locout #l1 ?{{{ l2, RET #l2; low l2 }}})%I.
+  Definition is_locin (locin : val) : iProp Σ :=
+    (∀ l2, {{{ low l2 }}} locin #l2 ?{{{ l1, RET #l1; True }}})%I.
+  Definition is_wrap (wrap : val) : iProp Σ :=
+    (∀ v1, {{{ inert v1 }}} wrap v1 ?{{{ v2, RET v2; low v2 }}})%I.
+
+  Lemma inert_membrane_spec p E locout locin :
+    {{{ is_locout locout ∗ is_locin locin }}}
+      membrane locout locin @ p; E
+    {{{ wrap, RET wrap; is_wrap wrap }}}.
+  Proof.
+    iIntros (Φ) "#(Hout & Hin)". rewrite -membrane_spec. clear Φ. iSplit.
+    - iIntros (l) "!#". iIntros (Φ) "_ HΦ".
+      by iApply ("Hout" $! l with "[] [$HΦ]").
+    - iIntros (l) "!#". iIntros (Φ) "Hl HΦ".
+      by iApply ("Hin" $! l with "[$Hl] [$HΦ]").
+  Qed.
+End inert.
